richerlang/typeSNScript.sml
@@ -1,0 +1,98 @@
+open HolKernel Parse boolLib bossLib;
+
+open richerLangTheory envSemTheory optionTheory finite_mapTheory;
+
+val _ = new_theory "typeSN";
+
+
+Definition sn_v_def:
+  (sn_v intT (IntV n) ⇔ T) ∧
+  (sn_v strT (StrV s) ⇔ T) ∧
+  (sn_v boolT (BoolV b) ⇔ T) ∧
+  (sn_v (fnT t1 t2) (Clos s e E) ⇔
+     ∀ v. sn_v t1 v ⇒ (∃ cl v'. eval_exp cl (E|+(s,v)) e = Value v' ∧ sn_v t2 v') ∨
+                      (∃ cl exn. eval_exp cl (E|+(s,v)) e = Exn exn)) ∧
+  (sn_v (pairT t1 t2) (PairV v1 v2) ⇔ sn_v t1 v1 ∧ sn_v t2 v2) ∧
+  (sn_v (sumT t1 t2) (SumLV v) ⇔ sn_v t1 v) ∧
+  (sn_v (sumT t1 t2) (SumRV v) ⇔ sn_v t2 v) ∧
+  (sn_v _ _ ⇔ F)
+Termination
+  WF_REL_TAC ‘inv_image (measure type_size) FST’
+End
+
+Definition envtype_sn_def:
+  envtype_sn G E ⇔
+    (* ∀ s ty. FLOOKUP G s = SOME ty ⇒ (∃ v. FLOOKUP E s = SOME v ∧ sn_v ty v) *)
+    ∀ s v. FLOOKUP E s = SOME v ⇒ (∃ ty. FLOOKUP G s = SOME ty ∧ sn_v ty v)
+End
+
+Definition sn_exec_def:
+  sn_exec t E e ⇔ (∃ cl v. eval_exp cl E e = Value v ∧ sn_v t v) ∨
+                  ∃ cl exn. eval_exp cl E e = Exn exn
+End
+
+Definition sn_e_def:
+  sn_e G t e ⇔
+    ∀ E. envtype_sn G E ⇒ sn_exec t E e
+End
+
+(*
+Theorem sn_v_value_type:
+  ∀ ty v. sn_v ty v ⇒ value_type v ty
+Proof
+  (* recInduct sn_v_ind >> simp[sn_v_def] >> rw[] >>
+  irule value_type_FnV >> *)
+  cheat
+QED
+
+Theorem envtype_sn_envtype:
+  envtype_sn G E ⇒ envtype G E
+Proof
+  metis_tac[envtype_sn_def, envtype_def, sn_v_value_type]
+QED
+*)
+
+Theorem sn_lemma:
+(* ∀ G e t. typecheck G e t ∧ free_vars e = FDOM G ⇒ sn_e G t e *)
+  ∀ G e t. typecheck G e t ⇒ sn_e G t e
+Proof
+  Induct_on ‘typecheck’ >> rw[sn_e_def, sn_v_def, eval_exp_def] >> gvs[AllCaseEqs(), PULL_EXISTS, result_bind_eq_value, sn_exec_def] >> rpt (first_x_assum $ drule_all_then $ strip_assume_tac) >~
+  [‘Fn s e’, ‘fnT dt rt’]
+  >- (rw[eval_exp_def] >> simp[sn_v_def] >> rpt strip_tac >> first_x_assum irule >>
+      simp[FLOOKUP_SIMP] >> rw[AllCaseEqs()]
+      >- (rename [‘FLOOKUP G s2 = SOME ty’] >>
+          ‘s2 ∈ FDOM G’ by metis_tac[flookup_thm] >>
+          ‘s2 ∈ free_vars e’ by ASM_SET_TAC [] >>
+          metis_tac[])
+      >> ASM_SET_TAC [])
+
+                                                                                     
+        
+  Induct_on ‘typecheck’ >> rw[sn_e_def, envtype_sn_def, sn_v_def, eval_exp_def] >> gvs[AllCaseEqs(), PULL_EXISTS, result_bind_eq_value, sn_exec_def] >> rpt (first_x_assum $ drule_all_then $ strip_assume_tac)
+  >- (rw[eval_exp_def])
+  >- (rw[eval_exp_def] >> DISJ1_TAC >> qexists ‘(cl+cl'+ cl'')’ >> rpt (dxrule clock_value_increment) >>
+      simp[] >> Cases_on ‘v''’ >> gvs[sn_v_def, AllCaseEqs()] >> metis_tac[])
+
+  >~ (rw[eval_exp_def] >> DISJ2_TAC >> qexists ‘cl''’ >> simp[]) >~
+  [‘If gd tb eb’, ‘eval_exp gc E gd = Value gv’,
+   ‘eval_exp tc E tb = Exn exn’, ‘eval_exp ec E eb = Value ev’]
+  >- (Cases_on ‘gv’ >> gvs[sn_v_def] >> rename [‘Value (BoolV bv)’] >>
+      Cases_on ‘bv’
+      >- (disj2_tac >> qexists ‘gc+tc’ >> rpt (dxrule clock_value_increment) >> rpt (dxrule clock_exn_increment) >> rw[eval_exp_def])
+      >> (disj1_tac >> qexists ‘gc+ec’ >> rpt (dxrule clock_value_increment) >> rw[eval_exp_def])) >~
+  [‘BinOp bop e1 e2’, ‘eval_exp c1 E e1 = Value v1’, ‘eval_exp c2 E e2 = Value v2’]
+  >- ( Cases_on ‘eval_bop bop v1 v2’
+       >- (disj1_tac >> rw[eval_exp_def] >> qexists ‘c1+c2’ >> rpt (dxrule clock_value_increment) >> rw[])) >~
+  [‘Fn s e’, ‘fnT dt rt’]
+  >- (rw[eval_exp_def] >> simp[sn_v_def] >> rpt strip_tac >> first_x_assum irule >>
+      simp[FLOOKUP_SIMP] >> rw[AllCaseEqs()]
+      >- (rename [‘FLOOKUP G s2 = SOME ty’] >>
+      ‘s2 ∈ FDOM G’ by metis_tac[flookup_thm] >>
+      ‘s2 ∈ free_vars e’ by ASM_SET_TAC [] >>
+      metis_tac[])
+      >> ASM_SET_TAC [])
+QED
+
+
+val _ = export_theory();
+
