semantics/proofs/deadlockFreedomScript.sml
@@ -13,23 +13,26 @@ Proof
   \\ rw [] \\ rw []
   (* IfThen *)
   >- (rename1 ‘IfThen v’
-     \\ Cases_on `FLOOKUP s' (v,s) = SOME [1w]`
+     \\ Cases_on `FLOOKUP s' (v,s) = SOME (BoolV T)`
      >- metis_tac [trans_if_true]
      \\ Cases_on `FLOOKUP s' (v,s)`
-     >- fs [no_undefined_vars_def,free_variables_def,FLOOKUP_DEF]
-     \\ metis_tac [trans_if_false])
+      >- fs [no_undefined_vars_def,free_variables_def,FLOOKUP_DEF]
+      >> Cases_on ‘x = (BoolV F)’
+      >- metis_tac [trans_if_false]
+      >> metis_tac [not_BoolV, trans_if_exn])
   (* Communication *)
   >- (rename1 ‘Com p1 v1 p2 v2’
      \\ `∃d. FLOOKUP s' (v1,p1) = SOME d`
-        by fs [no_undefined_vars_def,free_variables_def,FLOOKUP_DEF]
-     \\ metis_tac [trans_com,no_self_comunication_def])
+             by fs [no_undefined_vars_def,free_variables_def,FLOOKUP_DEF]
+      >> Cases_on ‘d’ 
+     \\ metis_tac [trans_com, trans_com_exn, no_self_comunication_def])
   (* Let *)
-  >- (rename1 ‘Let v p f’
+  >- (rename1 ‘Let v p e c’
       \\ `EVERY IS_SOME (MAP (FLOOKUP s') (MAP (λv. (v,p)) l))`
           by (last_assum mp_tac \\  rpt (pop_assum (K ALL_TAC))
               \\ rw [no_undefined_vars_def,free_variables_def]
               \\ Induct_on `l` \\ rw [IS_SOME_EXISTS,FLOOKUP_DEF])
-      \\ metis_tac [trans_let])
+      \\ metis_tac [trans_letval])
   (* Selection *)
   >- metis_tac [trans_sel,no_self_comunication_def]
   (* Recursion *)
